proof/server_proof/rpc.v
@@ -172,6 +172,88 @@ Lemma wp_Audit_cli_call (Q : cfg.t → state.t → iProp Σ)
   }}}.
 Proof. Admitted.
 
+Lemma wp_Start_cli_call (Q : cfg.t → state.t → iProp Σ)
+    c good sl_arg d0 (arg : list w8) ptr_reply (x : slice.t) :
+  {{{
+    is_pkg_init server ∗
+    "#His_cli" ∷ is_rpc_cli c good ∗
+    "Hsl_arg" ∷ sl_arg ↦*{d0} arg ∗
+    "Hptr_reply" ∷ ptr_reply ↦ x ∗
+    "#Hfupd" ∷ match good with None => True | Some γ =>
+      □ (|={⊤,∅}=> ∃ obj, own γ obj ∗ (own γ obj ={∅,⊤}=∗ Q γ obj)) end
+  }}}
+  c @ (ptrT.id advrpc.Client.id) @ "Call" server.StartRpc #sl_arg #ptr_reply
+  {{{
+    sl_reply err0, RET #err0;
+    "Hsl_arg" ∷ sl_arg ↦*{d0} arg ∗
+    "Hptr_reply" ∷ ptr_reply ↦ sl_reply ∗
+
+    "Herr_net" ∷ match err0 with true => True | false =>
+    ∃ replyB,
+    "Hsl_reply" ∷ sl_reply ↦* replyB ∗
+
+    "Hgood" ∷ match good with None => True | Some γ =>
+    ∃ chain vrf obj last_link,
+    let numEps := length obj.(state.hist) in
+    "%His_reply" ∷ ⌜StartReply.wish replyB (StartReply.mk' chain vrf) []⌝ ∗
+
+    "HQ" ∷ Q γ obj ∗
+    "%Hnoof_eps" ∷ ⌜numEps = sint.nat (W64 $ numEps)⌝ ∗
+
+    "%His_PrevEpochLen" ∷ ⌜uint.nat chain.(StartChain.PrevEpochLen) < numEps⌝ ∗
+    "#His_PrevLink" ∷ hashchain.is_chain
+      (take (uint.nat chain.(StartChain.PrevEpochLen)) obj.(state.hist).*1)
+      None chain.(StartChain.PrevLink)
+      (uint.nat chain.(StartChain.PrevEpochLen)) ∗
+    "%His_ChainProof" ∷ ⌜hashchain.wish_Proof chain.(StartChain.ChainProof)
+      (drop (uint.nat chain.(StartChain.PrevEpochLen)) obj.(state.hist).*1)⌝ ∗
+    "#His_last_link" ∷ hashchain.is_chain obj.(state.hist).*1 None
+      last_link numEps ∗
+    "#His_LinkSig" ∷ ktcore.wish_LinkSig γ.(cfg.sig_pk)
+      (W64 $ numEps - 1) last_link chain.(StartChain.LinkSig) ∗
+
+    "%Heq_VrfPk" ∷ ⌜γ.(cfg.vrf_pk) = vrf.(StartVrf.VrfPk)⌝ ∗
+    "#His_VrfPk" ∷ cryptoffi.is_vrf_pk vrf.(StartVrf.VrfPk) ∗
+    "#His_VrfSig" ∷ ktcore.wish_VrfSig γ.(cfg.sig_pk) γ.(cfg.vrf_pk)
+      vrf.(StartVrf.VrfSig)
+    end end
+  }}}.
+Proof. Admitted.
+
+Definition wish_CheckStartChain servPk chain digs cut (ep : w64) dig link : iProp Σ :=
+  ∃ digs0 digs1,
+  "#His_chain_prev" ∷ hashchain.is_chain digs0 cut chain.(server.StartChain.PrevLink)
+    (uint.nat chain.(server.StartChain.PrevEpochLen)) ∗
+  "%His_proof" ∷ ⌜hashchain.wish_Proof chain.(server.StartChain.ChainProof) digs1⌝ ∗
+  "#His_chain_start" ∷ hashchain.is_chain digs cut link
+    (uint.nat chain.(server.StartChain.PrevEpochLen) + length digs1) ∗
+  "#His_link_sig" ∷ ktcore.wish_LinkSig servPk ep link chain.(server.StartChain.LinkSig) ∗
+
+  "%Heq_digs" ∷ ⌜digs = digs0 ++ digs1⌝ ∗
+  "%Heq_ep" ∷ ⌜uint.Z ep = uint.Z chain.(server.StartChain.PrevEpochLen) + length digs1 - 1⌝ ∗
+  "%Heq_dig" ∷ ⌜last digs1 = Some dig⌝.
+
+Lemma wish_CheckStartChain_det pk c digs0 digs1 cut0 cut1 e0 e1 d0 d1 l0 l1 :
+  wish_CheckStartChain pk c digs0 cut0 e0 d0 l0 -∗
+  wish_CheckStartChain pk c digs1 cut1 e1 d1 l1 -∗
+  ⌜digs0 = digs1 ∧ cut0 = cut1 ∧ e0 = e1 ∧ d0 = d1 ∧ l0 = l1⌝.
+Proof.
+  iNamedSuffix 1 "0".
+  iNamedSuffix 1 "1".
+  iDestruct (hashchain.is_chain_inj with "His_chain_prev0 His_chain_prev1") as %[-> ->].
+  opose proof (hashchain.wish_Proof_det _ _ _ His_proof0 His_proof1) as ->.
+  simplify_eq/=.
+  iDestruct (hashchain.is_chain_det with "His_chain_start0 His_chain_start1") as %->.
+  iPureIntro.
+  rewrite -Heq_ep0 in Heq_ep1.
+  by simplify_eq/=.
+Qed.
+
+Definition wish_CheckStartVrf servPk vrf : iProp Σ :=
+  "#His_vrf_pk" ∷ cryptoffi.is_vrf_pk vrf.(server.StartVrf.VrfPk) ∗
+  "#His_vrf_sig" ∷ ktcore.wish_VrfSig servPk vrf.(server.StartVrf.VrfPk)
+    vrf.(server.StartVrf.VrfSig).
+
 Lemma wp_CallStart c good :
   {{{
     is_pkg_init server ∗
@@ -187,28 +269,69 @@ Lemma wp_CallStart c good :
       "#Hptr_vrf" ∷ StartVrf.own ptr_vrf vrf (□) ∗
 
       "Hgood" ∷ match good with None => True | Some γ =>
-        ∃ servHist last_link,
-        let numEps := length servHist in
+        ∃ servHist ep dig link,
         "#Hlb_servHist" ∷ mono_list_lb_own γ.(cfg.histγ) servHist ∗
-        "%Hnoof_eps" ∷ ⌜numEps = sint.nat (W64 $ numEps)⌝ ∗
-
-        "%His_PrevEpochLen" ∷ ⌜uint.nat chain.(StartChain.PrevEpochLen) < numEps⌝ ∗
-        "#His_PrevLink" ∷ hashchain.is_chain
-          (take (uint.nat chain.(StartChain.PrevEpochLen)) servHist.*1)
-          None chain.(StartChain.PrevLink)
-          (uint.nat chain.(StartChain.PrevEpochLen)) ∗
-        "%His_ChainProof" ∷ ⌜hashchain.wish_Proof chain.(StartChain.ChainProof)
-          (drop (uint.nat chain.(StartChain.PrevEpochLen)) servHist.*1)⌝ ∗
-        "#His_last_link" ∷ hashchain.is_chain servHist.*1 None
-          last_link numEps ∗
-        "#His_LinkSig" ∷ ktcore.wish_LinkSig γ.(cfg.sig_pk)
-          (W64 $ numEps - 1) last_link chain.(StartChain.LinkSig) ∗
-
-        "%Heq_VrfPk" ∷ ⌜γ.(cfg.vrf_pk) = vrf.(StartVrf.VrfPk)⌝ ∗
-        "#His_VrfSig" ∷ ktcore.wish_VrfSig γ.(cfg.sig_pk) γ.(cfg.vrf_pk)
-          vrf.(StartVrf.VrfSig) end)
+        "#wish_StartChain" ∷ wish_CheckStartChain γ.(cfg.sig_pk) chain
+          servHist.*1 None ep dig link ∗
+        "#Hwish_StartVrf" ∷ wish_CheckStartVrf γ.(cfg.sig_pk) vrf end)
     }}}.
-Proof. Admitted.
+Proof.
+  wp_start as "@". wp_auto.
+  wp_apply wp_alloc as "* Ha".
+  simpl in *.
+  wp_apply (wp_Start_cli_call (Q_read_lb [])
+    with "[$Ha]") as "* @".
+  { iFrame "#".
+    iDestruct (own_slice_nil DfracDiscarded) as "$".
+    case_match; try done.
+    iModIntro.
+    iMod mono_list_lb_own_nil as "#?".
+    by iApply op_read_lb. }
+  wp_if_destruct.
+  { rewrite ktcore.rw_BlameUnknown.
+    iApply "HΦ".
+    iSplit; [|by case_decide].
+    iPureIntro. apply ktcore.blame_unknown. }
+  iNamed "Herr_net".
+  iPersist "Hsl_reply".
+  wp_apply (StartReply.wp_dec with "[$Hsl_reply]") as "* Hgenie".
+  wp_if_destruct.
+  { rewrite ktcore.rw_BlameServFull.
+    iApply "HΦ".
+    iSplit; [|by case_decide].
+    iApply ktcore.blame_one.
+    iIntros (?).
+    case_match; try done.
+    iNamed "Hgood".
+    iApply "Hgenie".
+    naive_solver. }
+  iDestruct "Hgenie" as (??) "(#Hreply&_&%His_dec)".
+  destruct obj. iNamed "Hreply".
+  wp_auto. simpl.
+
+  rewrite ktcore.rw_BlameNone.
+  iApply "HΦ".
+  iSplit. { iPureIntro. apply ktcore.blame_none. }
+  case_decide; try done.
+  iFrame "#".
+  case_match; try done.
+  iNamed "Hgood".
+  opose proof (StartReply.wish_det _ _ _ _ His_dec His_reply) as [? _].
+  simplify_eq/=.
+  iDestruct "HQ" as "[#Hnew_hist %]".
+  rewrite Heq_VrfPk.
+  eremember (drop _ _) as digs1.
+  list_elem digs1 (pred $ length digs1) as dig.
+  { subst. len. }
+  subst.
+  rewrite -last_lookup in Hdig_lookup.
+  iFrame "#%".
+
+  repeat iSplit.
+  - iExactEq "His_last_link". rewrite /named. f_equal. len.
+  - by rewrite take_drop.
+  - len.
+Qed.
 
 End proof.
 End server.
